src/Prelude.v
@@ -1,10 +1,8 @@
 Require Stdlib.ZArith.BinIntDef Stdlib.PArith.BinPosDef Stdlib.NArith.BinNatDef.
 
-Notation "x :: l" := (cons x l)
-                     (at level 60, right associativity).
-Notation "[ ]" := nil.
-Notation "[ x ; .. ; y ]" := (cons x .. (cons y nil) ..).
-
 Number Notation BinNums.Z BinIntDef.Z.of_num_int BinIntDef.Z.to_num_int : Z_scope.
 Number Notation BinNums.positive BinPosDef.Pos.of_num_int BinPosDef.Pos.to_num_int : positive_scope.
 Number Notation BinNums.N BinNatDef.N.of_num_int BinNatDef.N.to_num_int : N_scope.
+
+Require Import List.
+Import ListNotations.
